prove first half of function calls in compile_val
cheating in function creation, because wanted to skip forward to
function calls to see if that works... now might be good to go back,
since this was unexpected given the simplifications made to Cv_bv.

compiler/correctness/compileCorrectnessScript.sml
@@ -1,4 +1,4 @@
-open HolKernel bossLib boolLib boolSimps SatisfySimps listTheory rich_listTheory pairTheory pred_setTheory finite_mapTheory alistTheory relationTheory arithmeticTheory lcsymtacs quantHeuristicsLib quantHeuristicsLibAbbrev
+open HolKernel bossLib boolLib boolSimps SatisfySimps listTheory rich_listTheory pairTheory pred_setTheory finite_mapTheory alistTheory relationTheory arithmeticTheory sortingTheory lcsymtacs quantHeuristicsLib quantHeuristicsLibAbbrev
 open MiniMLTerminationTheory miniMLExtraTheory miscTheory miscLib compileTerminationTheory intLangTheory bytecodeTerminationTheory evaluateEquationsTheory expToCexpTheory pmatchTheory labelClosuresTheory bytecodeEvalTheory bytecodeExtraTheory
 val _ = numLib.prefer_num()
 val _ = new_theory "compileCorrectness"
@@ -215,10 +215,7 @@ val (Cv_bv_rules,Cv_bv_ind,Cv_bv_cases) = Hol_reln`
    (LENGTH bvs = LENGTH recs + LENGTH envs) ∧
    (∀i x bv. i < LENGTH recs ∧ (x = EL i recs) ∧ (bv = EL i bvs) ⇒
      x < LENGTH defs ∧
-     ∃p jenv jdefs jx.
-       (bv = RefPtr p) ∧ jx < LENGTH jdefs ∧
-       (FLOOKUP rd.cls p = SOME (jenv,jdefs,jx)) ∧
-       syneq c (CRecClos jenv jdefs jx) (CRecClos env defs x)) ∧
+     ∃p. (bv = RefPtr p) ∧ (FLOOKUP rd.cls p = SOME (env,defs,x))) ∧
    (∀i x bv. i < LENGTH envs ∧ (x = EL i envs) ∧ (bv = EL (LENGTH recs + i) bvs) ⇒
        x < LENGTH env ∧ Cv_bv pp (EL x env) bv)
    ⇒ benv_bvs pp bvs cd env defs)`
@@ -284,6 +281,7 @@ val good_rd_def = Define`
       Cv_bv (mk_pp rd c bs) (CRecClos env defs j) (bs.refs ' p))
     rd.cls`
 
+(*
 val Cv_bv_syneq = store_thm("Cv_bv_syneq",
   ``(∀v1 bv. Cv_bv pp v1 bv ⇒ ∀v2. syneq (FST(SND pp)) v1 v2 ⇒ Cv_bv pp v2 bv) ∧
     (∀bvs cd env1 defs1. benv_bvs pp bvs cd env1 defs1 ⇒
@@ -363,6 +361,7 @@ val Cv_bv_syneq = store_thm("Cv_bv_syneq",
   first_x_assum match_mp_tac >>
   first_x_assum match_mp_tac >>
   simp[MEM_EL] >> metis_tac[])
+*)
 
 (*
 val syneq_exp_relates_same_vars = store_thm("syneq_exp_relates_same_vars",
@@ -2180,6 +2179,7 @@ val good_ecs_def = Define`
 
 val code_env_code_def = Define`
   code_env_code c code =
+  good_code_env c ∧
   ALL_DISTINCT (FILTER is_Label code) ∧
   FEVERY (λ(l,cd).
     ∃cs bc0 cc bc1.
@@ -2593,237 +2593,83 @@ val FDOM_bind_fv = store_thm("FDOM_bind_fv",
   metis_tac[])
 *)
 
-(*
 val Cenv_bs_bind_fv = store_thm("Cenv_bs_bind_fv",
-  ``∀c rd s env ns xs az i fvs bs
-     cenv defs e l vs a benv bve ret bvs st pp.
-    (env = DRESTRICT (extend_rec_env cenv cenv ns defs xs vs) fvs) ∧
-    (bs.stack = benv::CodePtr ret::(REVERSE bvs)++(Block closure_tag [CodePtr a;benv])::st) ∧
-    (pp = mk_pp rd c bs) ∧
+  ``∀c rd s env cenv bs pp cd e benv bve ret bvs a st vs fenv defs envs recs l.
+    (cenv = MAP CTEnv cd.ccenv) ∧
     (benv = Block 0 bve) ∧
-    (fvs = free_vars c e) ∧
-    benv_bvs pp bve fvs xs cenv defs ns i ∧
+    (bs.stack = benv::CodePtr ret::(REVERSE bvs)++(Block closure_tag [CodePtr a;benv])::st) ∧
+    (env = REVERSE vs ++ [CRecClos fenv defs cd.ix] ++ MAP (CRecClos fenv defs) recs ++ MAP (λn. EL n fenv) envs) ∧
+    (bind_fv (cd.az,e) cd.nz cd.ez cd.ix with body := cd.body = cd) ∧
+    (cd.ceenv = (recs,envs)) ∧
+    (pp = mk_pp rd c bs) ∧
+    (∀i l. i < LENGTH defs ∧ (EL i defs = INR l) ⇒
+        l ∈ FDOM c ∧ ((c ' l).nz = LENGTH defs) ∧
+        ((c ' l).ez = LENGTH fenv) ∧ ((c ' l).ix = i)) ∧
+    benv_bvs pp bve cd fenv defs ∧
     s_refs c rd s bs ∧
-    ALL_DISTINCT ns ∧
-    ALL_DISTINCT xs ∧
-    (ns ≠ [] ⇒ i < LENGTH ns ∧ (LENGTH ns = LENGTH defs) ∧ (EL i defs = (xs,INR l))) ∧
-    ((ns = []) ⇒ (defs = [(xs,INR l)])) ∧
-    (FLOOKUP c l = SOME e) ∧
+    cd.ix < LENGTH defs ∧
+    (EL cd.ix defs = INR l) ∧
+    (FLOOKUP c l = SOME cd) ∧
     (bc_find_loc_aux bs.code bs.inst_length l 0 = SOME a) ∧
-    (LENGTH xs = LENGTH vs) ∧
-    EVERY2 (Cv_bv pp) vs bvs ∧
-    fvs ⊆ FDOM cenv ∪ set ns ∪ set xs ∧
-    (az = LENGTH vs)
-    ⇒ Cenv_bs c rd s env (FST (ITSET (bind_fv ns xs az i) fvs (FEMPTY,0,[]))) 0 bs``,
-  rw[Cenv_bs_def] >>
-  simp[fmap_rel_def] >>
+    EVERY2 (Cv_bv pp) vs bvs ∧ (cd.az = LENGTH vs)
+    ⇒ Cenv_bs c rd s env cenv 0 bs``,
+  rw[Cenv_bs_def,closure_data_component_equality] >>
+  simp[EVERY2_EVERY] >>
   conj_asm1_tac >- (
-    rw[FDOM_bind_fv,FDOM_extend_rec_env,FDOM_DRESTRICT] >>
-    rw[INTER_COMM] >>
-    rw[GSYM SUBSET_INTER_ABSORPTION] ) >>
-  rfs[FDOM_bind_fv] >> pop_assum (assume_tac o SYM) >>
-  qabbrev_tac `fvs = free_vars c e` >>
-  `FINITE fvs` by rw[Abbr`fvs`] >>
-  qspecl_then[`ns`,`xs`,`LENGTH vs`,`i`,`fvs`,`(FEMPTY,0,[])`]mp_tac bind_fv_thm >>
-  rw[] >> simp[] >>
-  Cases_on `MEM x args` >- (
-    `MEM x xs` by (
-      fs[Abbr`args`,Abbr`fvl`,MEM_FILTER] ) >>
-    `∃n. (find_index x xs 1 = SOME (n + 1)) ∧ (EL n xs = x)` by (
-      simp[find_index_LEAST_EL] >>
-      numLib.LEAST_ELIM_TAC >>
-      fs[MEM_EL] >> PROVE_TAC[]) >>
-    Q.PAT_ABBREV_TAC`env1 = if X then Y else env0` >>
-    qho_match_abbrev_tac`P (env1 ' x)` >>
-    qsuff_tac`P (env0 ' x)` >- (
-      rw[Abbr`env1`,Abbr`P`,FAPPLY_FUPDATE_THM] >>
-      rw[] >> fs[] ) >>
-    `env0 ' x = (FEMPTY |++ ls1) ' x` by (
-      simp[Abbr`env0`] >>
-      match_mp_tac FUPDATE_LIST_APPLY_NOT_MEM_matchable >>
-      simp_tac std_ss [Abbr`ls2`,MAP_GENLIST,LIST_TO_SET_GENLIST,combinTheory.o_DEF,IMAGE_EL_count_LENGTH]>>
-      simp[Abbr`ecs`,FORALL_PROD,Abbr`envs`,Abbr`fvl`,MEM_MAP,MEM_FILTER] ) >>
-    pop_assum SUBST1_TAC >>
-    match_mp_tac FUPDATE_LIST_ALL_DISTINCT_APPLY_MEM >>
-    simp[RIGHT_EXISTS_AND_THM] >>
-    conj_tac >- rw[Abbr`ls1`,FILTER_ALL_DISTINCT,ALL_DISTINCT_SET_TO_LIST,Abbr`fvl`,MAP_ZIP,Abbr`args`] >>
-    simp[Abbr`ls1`,MAP_ZIP,Abbr`args`] >>
-    Q.PAT_ABBREV_TAC`ls = FILTER X fvl` >>
-    `ALL_DISTINCT ls` by rw[Abbr`ls`,FILTER_ALL_DISTINCT,Abbr`fvl`,ALL_DISTINCT_SET_TO_LIST] >>
-    simp[ALL_DISTINCT_MEM_ZIP_MAP,Abbr`P`] >>
-    fsrw_tac[ARITH_ss][EVERY2_EVERY,EVERY_MEM,FORALL_PROD] >>
-    rfs[MEM_ZIP] >> fsrw_tac[DNF_ss][] >>
-    simp[DRESTRICT_DEF] >>
-    simp[extend_rec_env_def,FOLDL2_FUPDATE_LIST,MAP2_MAP,FST_pair,MAP_ZIP,SND_pair] >>
-    Q.PAT_ABBREV_TAC`env2 = FOLDL X cenv ns` >>
-    qho_match_abbrev_tac`P ((env2 |++ ZIP (xs,vs)) ' x)` >>
-    match_mp_tac FUPDATE_LIST_ALL_DISTINCT_APPLY_MEM >>
-    simp[MAP_ZIP] >>
-    simp[MEM_ZIP] >>
-    fsrw_tac[DNF_ss][Abbr`P`] >>
-    qexists_tac`n`>>simp[]>>
-    imp_res_tac find_index_LESS_LENGTH >> rfs[] >>
-    Q.PAT_ABBREV_TAC`bv = EL X (Block 0 bve::Y)` >>
-    qsuff_tac`bv = EL n bvs` >- rw[] >>
-    rw[Abbr`bv`] >>
-    pop_assum mp_tac >>
-    rpt (pop_assum kall_tac) >>
-    simp[EL_CONS] >>
-    srw_tac[ARITH_ss][PRE_SUB1] >>
-    `(LENGTH bvs - n) = SUC (LENGTH bvs - n - 1)` by DECIDE_TAC >>
-    pop_assum SUBST1_TAC >> simp[] >>
-    simp[EL_APPEND1] >>
-    simp[EL_REVERSE,GSYM ADD1] ) >>
-  `¬MEM x xs` by (
-    rfs[Abbr`args`,MEM_FILTER,Abbr`fvl`,MEM_SET_TO_LIST] ) >>
-  Cases_on `find_index x ns 0 = SOME i` >- (
-    `x = EL i ns` by (
-      imp_res_tac find_index_ALL_DISTINCT_EL_eq >> fs[] ) >>
-    `ns ≠ []` by (Cases_on `ns` >> fs[find_index_def]) >>
-    `LENGTH bvs = LENGTH vs` by fs[EVERY2_EVERY] >>
-    fsrw_tac[ARITH_ss][ADD1] >>
-    `MEM (EL i ns) ns` by (rw[MEM_EL] >> PROVE_TAC[]) >>
-    simp[DRESTRICT_DEF] >>
-    simp[extend_rec_env_def,FOLDL_FUPDATE_LIST,FOLDL2_FUPDATE_LIST,MAP2_MAP,FST_pair,SND_pair,MAP_ZIP] >>
-    Q.PAT_ABBREV_TAC`env1 = cenv |++ X` >>
-    `(env1 |++ ZIP (xs,vs)) ' (EL i ns) = CRecClos cenv ns defs (EL i ns)` by (
-      match_mp_tac FUPDATE_LIST_APPLY_NOT_MEM_matchable >>
-      simp[MAP_ZIP,Abbr`env1`] >>
-      ho_match_mp_tac FUPDATE_LIST_ALL_DISTINCT_APPLY_MEM >>
-      simp[MAP_MAP_o,combinTheory.o_DEF,MEM_MAP] ) >>
-    pop_assum SUBST1_TAC >>
-    `LENGTH vs + 2 = SUC(SUC(LENGTH(REVERSE bvs)))` by srw_tac[ARITH_ss][ADD1] >>
-    pop_assum SUBST1_TAC >>
-    REWRITE_TAC[EL,TL] >>
+    qpat_assum`X = cd.ccenv`(SUBST1_TAC o SYM) >>
+    fsrw_tac[ARITH_ss][bind_fv_def,LET_THM] >>
+    srw_tac[ARITH_ss][]) >>
+  simp[EVERY_MEM,FORALL_PROD,MEM_ZIP,GSYM LEFT_FORALL_IMP_THM] >>
+  gen_tac >> strip_tac >>
+  simp[EL_MAP] >>
+  simp[option_case_NONE_F] >>
+  Cases_on`n< LENGTH vs` >- (
+    qpat_assum`X = cd.ccenv`(SUBST1_TAC o SYM) >>
+    simp[bind_fv_def,EL_APPEND1,EL_REVERSE,PRE_SUB1,el_check_def,ADD1] >>
+    fsrw_tac[ARITH_ss][EVERY2_EVERY] >>
+    simp[EL_CONS,PRE_SUB1,EL_APPEND1,EL_REVERSE] >>
+    fs[EVERY_MEM] >> rfs[MEM_ZIP,GSYM LEFT_FORALL_IMP_THM] >>
+    first_x_assum match_mp_tac >> simp[] ) >>
+  Cases_on`n = LENGTH vs` >- (
+    qpat_assum`X = cd.ccenv`(SUBST1_TAC o SYM) >>
+    simp[bind_fv_def] >>
     REWRITE_TAC[GSYM APPEND_ASSOC] >>
-    simp_tac std_ss [EL_LENGTH_APPEND,NULL,GSYM CONS_APPEND,HD] >>
-    simp[Once Cv_bv_cases] ) >>
-  Cases_on `MEM x ns` >- (
-    `ns ≠ []` by (Cases_on `ns` >> fs[]) >> fs[] >>
-    Cases_on `x = EL i ns` >- (
-      fs[] >>
-      `i < LENGTH ns` by rw[] >>
-      imp_res_tac find_index_ALL_DISTINCT_EL >>
-      fs[] ) >>
-    Q.PAT_ABBREV_TAC`env1 = if X then Y else env0` >>
-    qho_match_abbrev_tac`P (env1 ' x)` >>
-    qsuff_tac`P (env0 ' x)` >- (
-      rw[Abbr`env1`,Abbr`P`,FAPPLY_FUPDATE_THM] ) >>
-    simp[Abbr`env1`,Abbr`P`] >>
-    `∃jx. find_index x ns 0 = SOME jx` by (
-      metis_tac[find_index_MEM,optionTheory.NOT_SOME_NONE,optionTheory.option_CASES] ) >>
-    `MEM (x, CERef (jx + 1)) ecs` by (
-      simp[Abbr`ecs`,MEM_MAP,Abbr`envs`,MEM_FILTER,Abbr`fvl`] ) >>
-    `∃n. (env0 ' x = CTRef n) ∧ n < LENGTH ecs ∧ (EL n ecs = (x, CERef (jx + 1))) ∧ (find_index (EL n envs) ns 0 = SOME jx)` by (
-      fs[MEM_EL] >>
-      qmatch_assum_rename_tac`m < LENGTH ecs`[] >>
-      qexists_tac`m`>>simp[] >>
-      simp[Abbr`env0`] >>
-      reverse conj_tac >- (
-        fs[Abbr`ecs`] >> rfs[EL_MAP] >>
-        Cases_on`find_index (EL m envs) ns 0` >> fs[] ) >>
-      qabbrev_tac`fm = FEMPTY |++ ls1` >>
-      qho_match_abbrev_tac`P ((fm |++ ls2) ' (EL n ns))` >>
-      match_mp_tac FUPDATE_LIST_ALL_DISTINCT_APPLY_MEM >>
-      simp_tac std_ss [Abbr`ls2`,GENLIST_EL_MAP,MAP_GENLIST,combinTheory.o_DEF,LIST_TO_SET_GENLIST,IMAGE_EL_count_LENGTH,Abbr`P`] >>
-      conj_tac >- rw[FILTER_ALL_DISTINCT,Abbr`fvl`,ALL_DISTINCT_SET_TO_LIST,Abbr`ecs`,MAP_MAP_o,combinTheory.o_DEF,Abbr`envs`] >>
-      simp[] >>
-      qexists_tac`m` >>
-      qpat_assum`X = EL m ecs`(assume_tac o SYM) >>
-      simp[] ) >>
-    qpat_assum`benv_bvs pp bvs fvs xs cenv defs ns i`mp_tac >>
-    `envs ≠ []` by (
-      simp[Abbr`envs`,FILTER_EQ_NIL,combinTheory.o_DEF,EXISTS_MEM,Abbr`fvl`] >>
-      PROVE_TAC[] ) >>
-    simp[CONJUNCT2(SPEC_ALL Cv_bv_cases)] >>
-    disch_then strip_assume_tac >>
-    simp[] >>
-    `LENGTH ecs = LENGTH envs` by rw[Abbr`ecs`] >> fs[] >>
-    first_x_assum(qspec_then`n`mp_tac) >>
-    simp[] >>
-    disch_then(qx_choosel_then[`p`,`jenv`]strip_assume_tac) >>
-    fs[s_refs_def] >>
-    qpat_assum`good_rd c rd bs`(mp_tac o SIMP_RULE(srw_ss())[good_rd_def,FEVERY_DEF]) >>
-    strip_tac >>
-    first_x_assum(qspec_then`p`mp_tac) >>
-    fs[FLOOKUP_DEF] >>
-    simp[DRESTRICT_DEF,extend_rec_env_def,FOLDL_FUPDATE_LIST,FOLDL2_FUPDATE_LIST,MAP2_MAP,MAP_ZIP,FST_pair,SND_pair] >>
-    strip_tac >>
-    Q.PAT_ABBREV_TAC`env1 = cenv |++ X` >>
-    `(env1 |++ ZIP (xs,vs)) ' x = CRecClos cenv ns defs (EL jx ns)` by (
-      match_mp_tac FUPDATE_LIST_APPLY_NOT_MEM_matchable >>
-      simp[MAP_ZIP,Abbr`env1`] >>
-      ho_match_mp_tac FUPDATE_LIST_ALL_DISTINCT_APPLY_MEM >>
-      simp[MAP_MAP_o,combinTheory.o_DEF,MEM_MAP] >>
-      imp_res_tac find_index_ALL_DISTINCT_EL_eq >>
-      simp[]) >>
-    simp[] >>
-    match_mp_tac (MP_CANON syneq_Cv_bv) >> simp[] >>
-    qexists_tac`CRecClos jenv ns defs (EL jx ns)` >> simp[] >>
-    simp[syneq_cases] >>
-    fs[fmap_rel_OPTREL_FLOOKUP,EVERY_MEM,FORALL_PROD] >>
-    rpt gen_tac >> strip_tac >>
-    qx_gen_tac`v` >> strip_tac >>
-    first_x_assum(qspec_then`v`mp_tac) >>
-    rw[FLOOKUP_DRESTRICT] >>
-    fsrw_tac[DNF_ss][EXISTS_PROD,FORALL_PROD] >>
-    metis_tac[IN_DIFF] ) >>
-  `x ∈ set envs` by (
-    rw[MEM_FILTER,Abbr`envs`,Abbr`fvl`] ) >>
-  `ns ≠ [] ⇒ (MEM (EL i ns) ns)` by (
-    strip_tac >> fs[] >> rw[MEM_EL] >> PROVE_TAC[] ) >>
-  Q.PAT_ABBREV_TAC`env1 = if X then Y else env0` >>
-  qho_match_abbrev_tac`P (env1 ' x)` >>
-  qsuff_tac`P (env0 ' x)` >- (
-    rw[Abbr`env1`,Abbr`P`,FAPPLY_FUPDATE_THM] >>
-    rw[] >> fs[]) >>
-  simp[Abbr`env1`,Abbr`P`] >>
-  `find_index x ns 0 = NONE` by (
-    Q.ISPECL_THEN[`ns`,`x`,`0`]mp_tac find_index_MEM >> rw[] ) >>
-  `MEM (x, CEEnv x) ecs` by (
-    simp[Abbr`ecs`,MEM_MAP] ) >>
-  `∃n. (env0 ' x = CTEnv n) ∧ n < LENGTH ecs ∧ (EL n ecs = (x, CEEnv x)) ∧ (find_index (EL n envs) ns 0 = NONE) ∧ (x = EL n envs)` by (
-    fs[MEM_EL] >>
-    qmatch_assum_rename_tac`(x,CEEnv x) = EL m ecs`[] >>
-    `m = n` by (
-      fs[Abbr`ecs`] >> rfs[EL_MAP] >>
-      qsuff_tac `ALL_DISTINCT envs` >-
-        (fs[EL_ALL_DISTINCT_EL_EQ] >> PROVE_TAC[])>>
-      simp[Abbr`envs`,FILTER_ALL_DISTINCT,Abbr`fvl`,ALL_DISTINCT_SET_TO_LIST] ) >>
-    qexists_tac`n`>>simp[]>>
-    rfs[Abbr`env0`] >>
-    qabbrev_tac`fm = FEMPTY |++ ls1` >>
-    qho_match_abbrev_tac`P ((fm |++ ls2) ' (EL n envs))` >>
-    match_mp_tac FUPDATE_LIST_ALL_DISTINCT_APPLY_MEM >>
-    simp_tac std_ss [Abbr`ls2`,GENLIST_EL_MAP,MAP_GENLIST,combinTheory.o_DEF,LIST_TO_SET_GENLIST,IMAGE_EL_count_LENGTH,Abbr`P`] >>
-    conj_tac >- rw[FILTER_ALL_DISTINCT,Abbr`fvl`,ALL_DISTINCT_SET_TO_LIST,Abbr`ecs`,MAP_MAP_o,combinTheory.o_DEF,Abbr`envs`] >>
-    simp[] >>
-    qpat_assum`X = EL m ecs`(assume_tac o SYM) >>
-    qexists_tac`m`>>simp[]) >>
-  simp[] >>
-  qpat_assum`benv_bvs pp benv fvs xs cenv defs ns i`mp_tac >>
-  `envs ≠ []` by (
-    simp[Abbr`envs`,FILTER_EQ_NIL,combinTheory.o_DEF,EXISTS_MEM,Abbr`fvl`] >>
-    PROVE_TAC[] ) >>
-  simp[CONJUNCT2(SPEC_ALL Cv_bv_cases)] >>
-  disch_then(strip_assume_tac) >>
-  simp[] >>
-  `LENGTH ecs = LENGTH envs` by rw[Abbr`ecs`] >> fs[] >>
-  first_x_assum(qspec_then`n`mp_tac) >> simp[] >> rw[] >>
-  simp[DRESTRICT_DEF,extend_rec_env_def,FOLDL_FUPDATE_LIST,FOLDL2_FUPDATE_LIST,MAP2_MAP,MAP_ZIP,FST_pair,SND_pair] >>
-  `EL n envs ∈ FDOM cenv` by (
-    fsrw_tac[DNF_ss][SUBSET_DEF] >>
+    simp[EL_APPEND2,EL_APPEND1,el_check_def,ADD1,EL_CONS,PRE_SUB1] >>
+    fsrw_tac[ARITH_ss][EVERY2_EVERY] >>
+    REWRITE_TAC[GSYM APPEND_ASSOC] >>
+    simp[EL_APPEND2] >>
+    simp[Once Cv_bv_cases] >>
+    qexists_tac`cd` >>
+    qexists_tac`l` >>
+    simp[el_check_def] >>
     metis_tac[] ) >>
-  rw[] >>
-  Q.PAT_ABBREV_TAC`env1 = cenv |++ X` >>
-  `(env1 |++ ZIP (xs,vs)) ' (EL n envs) = cenv ' (EL n envs)` by (
-    match_mp_tac FUPDATE_LIST_APPLY_NOT_MEM_matchable >>
-    simp[MAP_ZIP,Abbr`env1`] >>
-    match_mp_tac EQ_SYM >>
-    match_mp_tac FUPDATE_LIST_APPLY_NOT_MEM_matchable >>
-    simp[MAP_MAP_o,combinTheory.o_DEF,MEM_MAP,FORALL_PROD] ) >>
-  rw[])
-*)
+  qpat_assum`X = cd.ccenv`(SUBST1_TAC o SYM) >>
+  simp[bind_fv_def] >>
+  REWRITE_TAC[GSYM APPEND_ASSOC] >>
+  simp[EL_APPEND2] >>
+  Q.PAT_ABBREV_TAC`lrecs = LENGTH (FILTER X Y)` >>
+  `lrecs = LENGTH recs` by (
+    fs[bind_fv_def,LET_THM,Abbr`lrecs`] >>
+    fsrw_tac[ARITH_ss][] ) >>
+  Cases_on`n < LENGTH vs + 1 + LENGTH recs` >- (
+    simp[EL_APPEND1,EL_MAP,el_check_def] >>
+    rator_x_assum`benv_bvs`mp_tac >>
+    simp[Once Cv_bv_cases] >> strip_tac >>
+    qpat_assum`∀i. i < LENGTH recs ⇒ X`(qspec_then`n - (LENGTH vs + 1)` mp_tac) >>
+    simp[] >> strip_tac >> simp[] >>
+    fs[FLOOKUP_DEF] >>
+    fs[s_refs_def,good_rd_def,FEVERY_DEF,UNCURRY] >>
+    qpat_assum`∀x. x ∈ FDOM rd.cls ⇒ X`(qspec_then`p`mp_tac) >>
+    simp[] ) >>
+  Q.PAT_ABBREV_TAC`lenvs = LENGTH (FILTER P (QSORT X Y))` >>
+  `lenvs = LENGTH envs` by (
+    fs[bind_fv_def,LET_THM,Abbr`lenvs`] >>
+    srw_tac[ARITH_ss][] ) >>
+  simp[EL_APPEND2,EL_GENLIST,EL_MAP,el_check_def] >>
+  rator_x_assum`benv_bvs`mp_tac >>
+  simp[Once Cv_bv_cases] >> strip_tac >>
+  qpat_assum`∀i. i < LENGTH envs ⇒ X`(qspec_then`n - (LENGTH recs + (LENGTH vs + 1))` mp_tac) >>
+  simp[] >> strip_tac >> simp[] )
 
 (*
 val benv_bvs_free_vars_SUBSET = store_thm("benv_bvs_free_vars_SUBSET",
@@ -2891,7 +2737,7 @@ val compile_val = store_thm("compile_val",
         BIGUNION (IMAGE all_Clocs (set s)) ⊆ count (LENGTH s) ∧
         (body_count exp = 0) ∧
         (res = (s', Rval v)) ∧
-        (bce ++ bcr = bs.code) ∧ good_code_env c bce ∧
+        (bce ++ bcr = bs.code) ∧ code_env_code c bce ∧
         (bs.pc = next_addr bs.inst_length bc0) ∧
         (free_vars exp ⊆ count (LENGTH cenv)) ∧
         Cenv_bs c rd s env cenv sz (bs with code := bce) ∧
@@ -2909,7 +2755,7 @@ val compile_val = store_thm("compile_val",
         ⇒
         ∀env0 defs vs klvs blvs benv ret args cl st.
         (az = LENGTH args) ∧ (lz = LENGTH klvs) ∧
-        (env = klvs ++ extend_rec_env env0 defs vs) ∧
+        (env = klvs ++ REVERSE vs ++ env0) ∧
         EVERY2 (Cv_bv (mk_pp rd c (bs with code := bce))) vs args ∧
         EVERY2 (Cv_bv (mk_pp rd c (bs with code := bce))) klvs blvs ∧
         (bs.stack = blvs++benv::CodePtr ret::(REVERSE args)++cl::st)
@@ -2922,7 +2768,7 @@ val compile_val = store_thm("compile_val",
         BIGUNION (IMAGE all_Clocs (set s)) ⊆ count (LENGTH s) ∧
         (body_count_list exps = 0) ∧
         (ress = (s', Rval vs)) ∧
-        (bce ++ bcr = bs.code) ∧ good_code_env c bce ∧
+        (bce ++ bcr = bs.code) ∧ code_env_code c bce ∧
         (bs.code = bc0 ++ code ++ bc1) ∧
         (bs.pc = next_addr bs.inst_length bc0) ∧
         (BIGUNION (IMAGE free_vars (set exps)) ⊆ count (LENGTH cenv)) ∧
@@ -3328,7 +3174,7 @@ val compile_val = store_thm("compile_val",
     simp[Once SWAP_REVERSE] >>
     `bs1.code = bs.code` by rw[Abbr`bs1`] >>
     fsrw_tac[ARITH_ss][] >>
-    disch_then(qspecl_then[`env0`,`defs`,`vs`]mp_tac) >>
+    disch_then(qspecl_then[`env0`,`vs`]mp_tac) >>
     simp[FUPDATE_LIST_THM] >>
     fsrw_tac[DNF_ss][] >>
     simp[Abbr`bs1`] >>
@@ -3378,8 +3224,8 @@ val compile_val = store_thm("compile_val",
       conj_tac >- (
         fsrw_tac[DNF_ss][MEM_EL] >>
         map_every qx_gen_tac[`l`,`i`] >> strip_tac >>
-        rator_x_assum`good_code_env`mp_tac >>
-        simp[good_code_env_def,FEVERY_DEF] >>
+        rator_x_assum`code_env_code`mp_tac >>
+        simp[code_env_code_def,good_code_env_def,FEVERY_DEF] >>
         strip_tac >> first_x_assum(qspec_then`l`mp_tac) >>
         `l ∈ FDOM c` by metis_tac[] >>
         `bs.code = bce ++ bcr` by metis_tac[] >>
@@ -3394,24 +3240,28 @@ val compile_val = store_thm("compile_val",
       simp[MEM_EL,GSYM LEFT_FORALL_IMP_THM] >>
       map_every qx_gen_tac[`l`,`i`] >> strip_tac >>
       simp[UNCURRY] >>
-      rator_x_assum`good_code_env`mp_tac >>
-      simp[good_code_env_def,FEVERY_DEF] >> strip_tac >>
-      first_x_assum(qspec_then`l`mp_tac) >>
+      rator_x_assum`code_env_code`mp_tac >>
+      simp[code_env_code_def,good_code_env_def,FEVERY_DEF] >> strip_tac >>
+      first_x_assum(qspec_then`c ' l`mp_tac) >>
+      simp[IN_FRANGE,GSYM LEFT_FORALL_IMP_THM] >>
+      disch_then(qspec_then`l`mp_tac) >> simp[] >>
       `l ∈ FDOM c` by metis_tac[] >>
-      simp[EVERY_MEM,MEM_EL,GSYM LEFT_FORALL_IMP_THM,closure_data_component_equality] >>
-
-      free_vars_mkshift
-      label_closures_thm
-      bind_fv_def
-
       `LENGTH cenv = LENGTH env` by metis_tac[Cenv_bs_def,EVERY2_EVERY] >>
+      `(c ' l).ez = LENGTH env` by metis_tac[] >>
+      simp[EVERY_MEM,MEM_EL,GSYM LEFT_FORALL_IMP_THM,closure_data_component_equality] >>
       strip_tac >>
-      conj_tac >- metis_tac[] >>
-      reverse conj_tac >- metis_tac[] >>
-      rator_x_assum`Cenv_bs`mp_tac >>
-      simp[Cenv_bs_def,EVERY2_EVERY,EVERY_MEM,FORALL_PROD,MEM_ZIP,GSYM LEFT_FORALL_IMP_THM] >>
-      simp[option_case_NONE_F] >>
-      metis_tac[optionTheory.IS_SOME_DEF] ) >>
+      conj_tac >- (
+        rator_x_assum`Cenv_bs`mp_tac >>
+        simp[Cenv_bs_def,EVERY2_EVERY,EVERY_MEM,FORALL_PROD,MEM_ZIP,GSYM LEFT_FORALL_IMP_THM] >>
+        simp[option_case_NONE_F] >>
+        metis_tac[optionTheory.IS_SOME_DEF] ) >>
+      qho_match_abbrev_tac`(∀n. n < LENGTH l2 ⇒ Q (EL n l2))` >>
+      qsuff_tac`EVERY Q l2` >- (
+        simp[EVERY_MEM,MEM_EL,GSYM LEFT_FORALL_IMP_THM] ) >>
+      simp[EVERY_MEM,Abbr`Q`] >>
+      qpat_assum`(c ' l).ceenv = X`mp_tac >>
+      simp[bind_fv_def,Abbr`l2`,MEM_FILTER,MEM_MAP,QSORT_MEM,MEM_GENLIST] >>
+      metis_tac[]) >>
     disch_then(Q.X_CHOOSE_THEN`rs`strip_assume_tac) >>
     qmatch_assum_abbrev_tac`bc_next^* bs bs1` >>
     qabbrev_tac`rd' = rd with cls := rd.cls |++ (GENLIST (λi. (EL i rs, (env, defs, i))) (LENGTH rs))` >>
@@ -3468,7 +3318,7 @@ val compile_val = store_thm("compile_val",
           conj_asm2_tac >- (
             qsuff_tac`MEM (Label l) bce` >- (
               metis_tac[bc_find_loc_aux_append_code,bc_find_loc_aux_NONE,optionTheory.option_CASES,optionTheory.THE_DEF] ) >>
-            fs[good_code_env_def,FEVERY_DEF] >>
+            fs[code_env_code_def,good_code_env_def,FEVERY_DEF] >>
             first_x_assum(qspec_then`l`mp_tac)>>
             first_x_assum(qspec_then`l`mp_tac)>>
             rw[] >> simp[] ) >>
@@ -3479,12 +3329,35 @@ val compile_val = store_thm("compile_val",
           map_every qexists_tac[`envs`,`recs`] >>
           simp[] >>
           conj_tac >- metis_tac[FST,SND,pair_CASES] >>
-          reverse conj_tac >- (
+          conj_tac >- (
             gen_tac >> strip_tac >>
-            simp[EL_APPEND2,EL_MAP] >>
-            Cenv_bs_def
-            s_refs_def
-
+            fs[code_env_code_def,good_code_env_def] >>
+            first_x_assum(qspec_then`c ' l`mp_tac) >>
+            simp[IN_FRANGE,GSYM LEFT_FORALL_IMP_THM] >>
+            disch_then(qspec_then`l`mp_tac) >>
+            simp[closure_data_component_equality] >>
+            simp[bind_fv_def] >> strip_tac >> fs[] >>
+            simp[EL_APPEND1,EL_MAP] >>
+            conj_asm1_tac >- (
+              qsuff_tac `EVERY (λn. n < (c ' l).nz) recs` >- (
+                simp[EVERY_MEM,MEM_EL,GSYM LEFT_FORALL_IMP_THM] >>
+                metis_tac[] ) >>
+              simp[Abbr`recs`,EVERY_MEM,MEM_FILTER,MEM_GENLIST] ) >>
+            simp[FLOOKUP_DEF,Abbr`rd'`,FDOM_FUPDATE_LIST,MEM_MAP,MEM_GENLIST,EXISTS_PROD] >>
+            conj_tac >- metis_tac[] >>
+            qho_match_abbrev_tac`(fm |++ ls) ' k = X` >>
+            qho_match_abbrev_tac`P ((fm |++ ls) ' k)` >>
+            ho_match_mp_tac FUPDATE_LIST_ALL_DISTINCT_APPLY_MEM >>
+            `MAP FST ls = rs` by (
+              simp[LIST_EQ_REWRITE,Abbr`ls`,EL_MAP] ) >>
+            simp[] >>
+            simp[MEM_EL,Abbr`ls`,Abbr`P`] >>
+            qexists_tac`EL i recs` >>
+            simp[Abbr`k`] ) >>
+          gen_tac >> strip_tac >>
+          simp[EL_APPEND2,EL_MAP] >>
+          cheat
+          (*
           qpat_assum`good_ecs X Y`mp_tac >>
           simp[good_ecs_def,FEVERY_DEF] >>
           first_x_assum(qspecl_then[`xs`,`l`,`n`]mp_tac) >>
@@ -3551,12 +3424,11 @@ val compile_val = store_thm("compile_val",
           Q.PAT_ABBREV_TAC`z = LENGTH defs - y`  >>
           qexists_tac`z` >>
           simp[Abbr`z`,Abbr`Q`] >>
-          simp[Abbr`P`] ) >>
+          simp[Abbr`P`] *) ) >>
         match_mp_tac Cenv_bs_change_store >>
         Q.PAT_ABBREV_TAC`pc = next_addr il X` >>
         map_every qexists_tac[`rd`,`s`,`bs with <| pc := pc ; code := bce|>`] >>
         simp[bc_state_component_equality,Abbr`rd'`,Cenv_bs_with_pc] >>
-        `LENGTH bvs = LENGTH rs` by rw[Abbr`bvs`] >>
         fs[Cenv_bs_def,s_refs_def] >>
         reverse conj_tac >- (
           simp[SUBMAP_DEF,DRESTRICT_DEF,FDOM_FUPDATE_LIST] >>
@@ -3564,14 +3436,16 @@ val compile_val = store_thm("compile_val",
           match_mp_tac EQ_SYM >>
           match_mp_tac FUPDATE_LIST_APPLY_NOT_MEM >>
           simp[MAP_ZIP] >>
-          fs[f_o_f_DEF,EXTENSION] >>
           metis_tac[] ) >>
         fs[Cenv_bs_def,s_refs_def,fmap_rel_def,good_rd_def] >>
         conj_tac >- (
           fs[FEVERY_DEF,UNCURRY,FDOM_FUPDATE_LIST] >>
           simp[MAP_GENLIST,combinTheory.o_DEF,MAP_ZIP,MEM_GENLIST] >>
           qx_gen_tac`x` >>
+          Q.ISPECL_THEN[`rs`,`x`](mp_tac o SYM)MEM_EL >>
+          simp[] >> disch_then kall_tac >>
           Cases_on`MEM x rs` >> simp[] >- (
+            cheat (*
             disch_then kall_tac >>
             conj_tac >- (
               fs[f_o_f_DEF,EXTENSION,IN_FRANGE] >>
@@ -3597,28 +3471,20 @@ val compile_val = store_thm("compile_val",
             qho_match_abbrev_tac`P ((bs.refs |++ ls) ' k)` >>
             match_mp_tac FUPDATE_LIST_ALL_DISTINCT_APPLY_MEM >>
             simp[Abbr`ls`,MAP_ZIP,Abbr`P`,Abbr`X`,MEM_ZIP,Abbr`k`] >>
-            qexists_tac`i`>>simp[EL_REVERSE,PRE_SUB1]) >>
-          reverse strip_tac >- metis_tac[MEM_EL] >>
+            qexists_tac`i`>>simp[EL_REVERSE,PRE_SUB1]*) ) >>
           Q.PAT_ABBREV_TAC`bv = (bs.refs |++ ls) ' x` >>
           Q.PAT_ABBREV_TAC`dd = (rd.cls |++ ls) ' x` >>
           qsuff_tac`(bv = bs.refs ' x) ∧ (dd = rd.cls ' x)` >- (
-            strip_tac >>
-            conj_tac >- metis_tac[] >>
-            conj_tac >- metis_tac[] >>
-            conj_tac >- metis_tac[] >>
+            ntac 2 strip_tac >>
             match_mp_tac (MP_CANON (GEN_ALL (CONJUNCT1 (SPEC_ALL Cv_bv_SUBMAP)))) >> simp[] >>
-            qexists_tac`rd` >> simp[] ) >>
+            qexists_tac`rd` >> simp[] >> rfs[]) >>
           map_every qunabbrev_tac[`bv`,`dd`] >>
           conj_tac >>
           match_mp_tac FUPDATE_LIST_APPLY_NOT_MEM >>
           simp[MAP_ZIP,MAP_GENLIST,combinTheory.o_DEF] >>
           TRY (qmatch_abbrev_tac `x ∉ set rs'` >> `rs = rs'` by lrw[Abbr`rs'`,LIST_EQ_REWRITE]) >>
           metis_tac[] ) >>
-        conj_asm1_tac >- (
-          fs[f_o_f_DEF,EXTENSION,FDOM_FUPDATE_LIST,MAP_ZIP] >>
-          metis_tac[] ) >>
-        simp[f_o_f_DEF] >>
-        qx_gen_tac `x` >> strip_tac >>
+        cheat (*
         qsuff_tac`rd.sm ' x ∉ set (MAP FST (ZIP (rs,REVERSE bvs)))` >- (
           strip_tac >>
           simp[FUPDATE_LIST_APPLY_NOT_MEM,f_o_f_DEF] >>
@@ -3627,24 +3493,21 @@ val compile_val = store_thm("compile_val",
           metis_tac[f_o_f_DEF] ) >>
         simp[MAP_ZIP] >>
         fs[f_o_f_DEF,EXTENSION] >>
-        metis_tac[] ) >>
+        metis_tac[] *) ) >>
       fs[GSYM FILTER_EQ_NIL,combinTheory.o_DEF] >>
       simp[ALL_DISTINCT_APPEND,FILTER_APPEND,Abbr`ccs`] ) >>
     simp[] >>
-    map_every qunabbrev_tac[`P`,`Q`,`R`] >>
     strip_tac >>
     conj_tac >- (
       pop_assum kall_tac >>
       pop_assum mp_tac >>
-      Q.PAT_ABBREV_TAC`cenv1 = cenv |++ ls` >>
-      qspecl_then[`cd`,`cenv1`,`TCNonTail F`,`sz + LENGTH ns`,`ccs`,`exp`](Q.X_CHOOSE_THEN`ce`strip_assume_tac)(CONJUNCT1 compile_append_out) >>
+      Q.PAT_ABBREV_TAC`cenv1 = ls ++ cenv` >>
+      qspecl_then[`c`,`cenv1`,`TCNonTail F`,`sz + LENGTH defs`,`ccs`,`exp`](Q.X_CHOOSE_THEN`ce`strip_assume_tac)(CONJUNCT1 compile_append_out) >>
       disch_then(qspec_then`REVERSE ce`mp_tac) >>
-      qspecl_then[`cd`,`cenv`,`TCNonTail F`,`sz`,`exp`,`0`,`ccs`,`ns`](Q.X_CHOOSE_THEN`cb`strip_assume_tac)(CONJUNCT1(CONJUNCT2 compile_append_out)) >>
+      qspecl_then[`c`,`cenv`,`TCNonTail F`,`sz`,`exp`,`0`,`ccs`,`LENGTH defs`](Q.X_CHOOSE_THEN`cb`strip_assume_tac)(CONJUNCT1(CONJUNCT2 compile_append_out)) >>
       `bs1.code = bs.code` by rw[Abbr`bs1`] >>
-      qspecl_then[`cd`,`cenv`,`TCNonTail F`,`sz`,`exp`,`0`,`ccs`,`ns`]mp_tac compile_bindings_thm >>
+      qspecl_then[`c`,`cenv`,`TCNonTail F`,`sz`,`exp`,`0`,`ccs`,`LENGTH defs`]mp_tac compile_bindings_thm >>
       simp[Once SWAP_REVERSE] >>
-      Q.PAT_ABBREV_TAC`cenv2 = cenv |++ ls` >>
-      `(cenv2 = cenv1)` by ( simp[Abbr`cenv1`,Abbr`cenv2`] ) >>
       qpat_assum`X = ce ++ ccs.out`mp_tac >>
       simp[] >> strip_tac >> strip_tac >>
       strip_tac >> gen_tac >> strip_tac >>
@@ -3682,7 +3545,7 @@ val compile_val = store_thm("compile_val",
       fs[Abbr`rd'`] >>
       reverse conj_tac >- metis_tac[SUBMAP_TRANS] >>
       match_mp_tac SUBMAP_TRANS >>
-      qexists_tac`DRESTRICT bs1.refs (COMPL (FRANGE rd.sm))` >>
+      qexists_tac`DRESTRICT bs1.refs (COMPL (set rd.sm))` >>
       simp[] >>
       simp[SUBMAP_DEF,DRESTRICT_DEF] >>
       rw[] >- (
@@ -3696,58 +3559,33 @@ val compile_val = store_thm("compile_val",
       simp[Abbr`bs1`,FDOM_FUPDATE_LIST] ) >>
     pop_assum mp_tac >>
     pop_assum kall_tac >>
-    Q.PAT_ABBREV_TAC`cenv1 = cenv |++ ls` >>
+    Q.PAT_ABBREV_TAC`cenv1 = ls ++ cenv` >>
     strip_tac >>
     rpt gen_tac >>
-    pop_assum(mp_tac o Q.SPECL[`lz + LENGTH (ns:string list)`,`az`] o CONV_RULE (RESORT_FORALL_CONV List.rev)) >>
-    qspecl_then[`cd`,`cenv1`,`TCTail az (lz + LENGTH ns)`,`sz + LENGTH ns`,`ccs`,`exp`](Q.X_CHOOSE_THEN`ce`strip_assume_tac)(CONJUNCT1 compile_append_out) >>
+    pop_assum(mp_tac o Q.SPECL[`lz + LENGTH (defs:def list)`,`az`] o CONV_RULE (RESORT_FORALL_CONV List.rev)) >>
+    qspecl_then[`c`,`cenv1`,`TCTail az (lz + LENGTH defs)`,`sz + LENGTH defs`,`ccs`,`exp`](Q.X_CHOOSE_THEN`ce`strip_assume_tac)(CONJUNCT1 compile_append_out) >>
     disch_then(qspec_then`REVERSE ce`mp_tac o CONV_RULE SWAP_FORALL_CONV) >>
-    qspecl_then[`cd`,`cenv`,`TCTail az lz`,`sz`,`exp`,`0`,`ccs`,`ns`](Q.X_CHOOSE_THEN`cb`strip_assume_tac)(CONJUNCT1(CONJUNCT2 compile_append_out)) >>
+    qspecl_then[`c`,`cenv`,`TCTail az lz`,`sz`,`exp`,`0`,`ccs`,`LENGTH defs`](Q.X_CHOOSE_THEN`cb`strip_assume_tac)(CONJUNCT1(CONJUNCT2 compile_append_out)) >>
     `bs1.code = bs.code` by rw[Abbr`bs1`] >>
-    qspecl_then[`cd`,`cenv`,`TCTail az lz`,`sz`,`exp`,`0`,`ccs`,`ns`]mp_tac compile_bindings_thm >>
+    qspecl_then[`c`,`cenv`,`TCTail az lz`,`sz`,`exp`,`0`,`ccs`,`LENGTH defs`]mp_tac compile_bindings_thm >>
     simp[Once SWAP_REVERSE] >>
-    Q.PAT_ABBREV_TAC`cenv2 = cenv |++ ls` >>
-    `(cenv2 = cenv1)` by ( simp[Abbr`cenv1`,Abbr`cenv2`] ) >>
     qpat_assum`X = ce ++ ccs.out`mp_tac >>
     simp[] >> strip_tac >> strip_tac >>
     strip_tac >> strip_tac >>
     rpt (qpat_assum`∀j k. (TCTail az lz = X) ⇒ Y`kall_tac) >>
     rfs[] >> fs[] >> rw[] >>
     fs[FOLDL_FUPDATE_LIST] >>
-    first_x_assum(qspecl_then[`env0`,`ns'`,`defs'`,`xs`,`vs`]mp_tac) >>
-    Q.PAT_ABBREV_TAC`klvs2 = MAP (X:string->string#Cv) ns` >>
+    first_x_assum(qspecl_then[`env0`,`vs`]mp_tac) >>
+    Q.PAT_ABBREV_TAC`klvs2:Cv list = GENLIST X Y` >>
     qpat_assum`Abbrev(bs1 = X)`mp_tac >>
-    Q.PAT_ABBREV_TAC`bvs:bc_value list = REVERSE (MAP X defs)` >>
+    Q.PAT_ABBREV_TAC`bvs:bc_value list = (MAP X defs)` >>
     strip_tac >>
-    disch_then(qspecl_then[`(REVERSE klvs2)++klvs`,`bvs++blvs`]mp_tac) >>
+    disch_then(qspecl_then[`klvs2++klvs`,`bvs++blvs`]mp_tac) >>
     simp[Abbr`bs1`] >>
     disch_then(qspec_then`args`mp_tac) >>
     simp[] >>
-    qmatch_abbrev_tac`(P ⇒ Q) ⇒ R` >>
-    `P` by (
-      map_every qunabbrev_tac[`P`,`Q`,`R`] >>
+    discharge_hyps >- (
       conj_tac >- simp[Abbr`klvs2`] >>
-      conj_tac >- (
-        fs[DISJOINT_SYM,MAP_REVERSE] >>
-        simp[Abbr`klvs2`,MAP_MAP_o,combinTheory.o_DEF] >>
-        qpat_assum`DISJOINT (FDOM cenv1) X`mp_tac >>
-        simp[Abbr`cenv1`,FDOM_FUPDATE_LIST,MAP_ZIP,DISJOINT_SYM] ) >>
-      conj_asm1_tac >- (
-        simp[Abbr`klvs2`,MAP_MAP_o,combinTheory.o_DEF,ALL_DISTINCT_APPEND,MAP_REVERSE,ALL_DISTINCT_REVERSE] >>
-        fs[DISJOINT_DEF,EXTENSION] >>
-        metis_tac[] ) >>
-      conj_tac >- (
-        simp[FUPDATE_LIST_APPEND] >>
-        qmatch_abbrev_tac`fm |++ l1 |++ l2 = X` >>
-        match_mp_tac EQ_TRANS >>
-        qexists_tac `fm |++ l2 |++ l1` >>
-        conj_tac >- (
-          match_mp_tac FUPDATE_LIST_APPEND_COMMUTES >>
-          fs[ALL_DISTINCT_APPEND,DISJOINT_DEF,EXTENSION,Abbr`l1`,Abbr`l2`,MAP_REVERSE] >>
-          metis_tac[] ) >>
-        AP_THM_TAC >> AP_TERM_TAC >>
-        match_mp_tac FUPDATE_LIST_ALL_DISTINCT_PERM >>
-        simp[Abbr`l2`,Abbr`klvs2`,MAP_MAP_o,combinTheory.o_DEF] ) >>
       conj_tac >- (
         fs[EVERY2_EVERY,EVERY_MEM,FORALL_PROD] >>
         `rd'.sm = rd.sm` by rw[Abbr`rd'`] >>
@@ -3761,10 +3599,15 @@ val compile_val = store_thm("compile_val",
         simp[EVERY_MEM,FORALL_PROD,MEM_ZIP] >>
         srw_tac[DNF_ss][EL_MAP,Abbr`klvs2`,EL_REVERSE,PRE_SUB1] >>
         fs[Cenv_bs_def,s_refs_def,good_rd_def,FEVERY_DEF,Abbr`rd'`] >>
+        cheat
+        (*
         first_x_assum(qspec_then`EL n rs`mp_tac) >>
         simp[FDOM_FUPDATE_LIST,MAP_GENLIST,combinTheory.o_DEF,MEM_GENLIST,MAP_ZIP] >>
         `MEM (EL n rs) rs` by metis_tac[MEM_EL] >>
-        simp[] >>
+        simp[] >> strip_tac >>
+        simp[Once Cv
+        qunabbrev_tac`bvs`
+        simp[Abbr`bvs`]
         simp[TAKE_LENGTH_ID_rwt] >>
         qmatch_abbrev_tac`(P ⇒ Q) ⇒ R` >>
         `P` by (
@@ -3785,12 +3628,12 @@ val compile_val = store_thm("compile_val",
         simp[MEM_ZIP] >>
         srw_tac[DNF_ss][Abbr`Q`] >>
         qexists_tac`n`>>simp[Abbr`R`] >>
-        simp[EL_MAP] ) >>
+        simp[EL_MAP] *)) >>
       fs[EVERY_MEM,FORALL_PROD] >> rw[] >>
       match_mp_tac (MP_CANON (GEN_ALL (CONJUNCT1 (SPEC_ALL Cv_bv_SUBMAP)))) >> simp[] >>
       qexists_tac`rd` >> simp[] >>
       simp[Abbr`rd'`] ) >>
-    simp[Abbr`Q`,Abbr`R`,code_for_return_def] >>
+    simp[code_for_return_def] >>
     asm_simp_tac(srw_ss()++DNF_ss)[] >>
     map_every qx_gen_tac[`bv1`,`rf1`,`rd1`] >>
     strip_tac >>
@@ -3816,23 +3659,21 @@ val compile_val = store_thm("compile_val",
   strip_tac >- (
     rpt gen_tac >> strip_tac >>
     rpt gen_tac >>
-    Cases_on`cb`>>fs[] >>
+    Cases_on`cb`>>TRY(PairCases_on`x`)>>fs[] >>
     strip_tac >>
     simp[compile_def,pushret_def] >>
     qmatch_assum_rename_tac`l ∈ FDOM c`[] >>
     conj_asm1_tac >- (
       simp[code_for_push_def] >>
-      Q.ISPECL_THEN[`cd`,`cenv`,`sz`,`0`,`cs`,`[(xs,INR l)]:def list`]mp_tac compile_closures_thm >>
+      Q.ISPECL_THEN[`c`,`cenv`,`sz`,`cs`,`[INR l]:def list`]mp_tac compile_closures_thm >>
       simp[] >> disch_then(Q.X_CHOOSE_THEN`cx`strip_assume_tac) >>
       simp[] >>
       fsrw_tac[DNF_ss][] >> rw[] >>
       first_x_assum(qspecl_then[`bs`,`bc0`,`bc1`,`FDOM rd.cls`]mp_tac) >>
-      qmatch_abbrev_tac`(P ⇒ Q) ⇒ R` >>
-      `P` by (
-        map_every qunabbrev_tac[`P`,`Q`,`R`] >>
+      discharge_hyps >- (
         simp[] >>
         conj_tac >- (
-          fs[good_code_env_def,FEVERY_DEF] >>
+          fs[code_env_code_def,good_code_env_def,FEVERY_DEF] >>
           first_x_assum(qspec_then`l`mp_tac) >>
           rw[] >>
           simp[bc_find_loc_def] >>
@@ -3844,51 +3685,37 @@ val compile_val = store_thm("compile_val",
           pop_assum mp_tac >>
           qpat_assum`X ++ Y = bc0 ++ cx ++ bc1`(SUBST1_TAC o SYM) >>
           simp[] ) >>
-        fs[good_ecs_def,FEVERY_DEF,FLOOKUP_DEF] >> rfs[] >>
-        first_x_assum(qspec_then`l`mp_tac) >>
-        simp[] >> strip_tac >>
-        qspecl_then[`[]`,`xs`,`LENGTH xs`,`0`,`free_vars (c \\ l) (c ' l)`,`(FEMPTY,0,[])`]mp_tac bind_fv_thm >>
-        simp[] >> strip_tac >>
-        simp[MEM_MAP,FORALL_PROD,EXISTS_PROD,MEM_FILTER] >>
+        fs[code_env_code_def,good_code_env_def] >> rfs[] >>
+        first_x_assum(qspec_then`c ' l`mp_tac) >>
+        simp[IN_FRANGE,GSYM LEFT_FORALL_IMP_THM] >>
+        disch_then(qspec_then`l`mp_tac) >>
+        `LENGTH cenv = LENGTH env` by fs[Cenv_bs_def,EVERY2_EVERY] >>
+        simp[closure_data_component_equality,UNCURRY] >>
+        strip_tac >>
+        reverse conj_tac >- (
+          fs[bind_fv_def,LET_THM] ) >>
         ntac 2 (pop_assum kall_tac) >>
-        conj_tac >- (
-          simp[GSYM FORALL_AND_THM] >>
-          simp[GSYM IMP_CONJ_THM] >>
-          rpt gen_tac >> strip_tac >>
-          fsrw_tac[DNF_ss][SUBSET_DEF] >>
-          qpat_assum`CEEnv fv = X`mp_tac >>
-          BasicProvers.CASE_TAC >> fs[] >>
-          rw[] >>
-          fs[Cenv_bs_def,fmap_rel_def] >>
-          first_x_assum(qspec_then`fv`mp_tac) >>
-          fs[FDOM_DRESTRICT] >>
-          `fv ∈ FDOM env` by (
-            fsrw_tac[DNF_ss][EXTENSION] >>
-            metis_tac[] ) >>
-          simp[] >>
-          Q.PAT_ABBREV_TAC`P = lookup_ct x y z a b` >>
-          Cases_on`P`>>rw[] ) >>
-        rw[] >>
-        simp[find_index_def] ) >>
-      simp[] >>
-      map_every qunabbrev_tac[`P`,`Q`,`R`] >>
+        fs[EVERY_MEM] >>
+        rator_x_assum`Cenv_bs`mp_tac >>
+        simp[Cenv_bs_def,EVERY2_EVERY,EVERY_MEM,FORALL_PROD,MEM_ZIP,GSYM LEFT_FORALL_IMP_THM,option_case_NONE_F] >>
+        metis_tac[optionTheory.IS_SOME_DEF] ) >>
       disch_then(Q.X_CHOOSE_THEN`rs`strip_assume_tac) >>
       rfs[LENGTH_NIL,FUPDATE_LIST_THM] >> rw[] >>
       pop_assum mp_tac >>
       Q.PAT_ABBREV_TAC`bv = Block 3 X` >>
       strip_tac >>
-      map_every qexists_tac[`bs.refs`,`rd`,`bv`] >>
+      map_every qexists_tac[`bs.refs |++ ZIP (rs,[bv])`,`rd`,`bv`] >>
       simp[] >>
       conj_tac >- (
-        simp[Once Cv_bv_cases] >>
+        simp[Once Cv_bv_cases,el_check_def,Abbr`bv`,UNCURRY,FLOOKUP_DEF]>>
+        qpat_assum`bs.code = X`kall_tac >>
+        qpat_assum`X = bs.code`(assume_tac o SYM) >>
+        qexists_tac`l`>>simp[bc_find_loc_def] >>
         `MEM (Label l) bce` by (
-          fs[good_code_env_def,FEVERY_DEF] >>
-          first_x_assum(qspec_then`l`mp_tac) >>
+          fs[code_env_code_def,good_code_env_def,FEVERY_DEF] >>
+          last_x_assum(qspec_then`l`mp_tac) >>
           simp[] >> rw[] >> simp[] ) >>
-        simp[Abbr`bv`] >>
-        qpat_assum`bs.code = bc0 ++ Y`kall_tac >>
         qpat_assum`bc_next^* X Y`kall_tac >>
-        fs[UNCURRY,FLOOKUP_DEF,bc_find_loc_def] >>
         conj_tac >- (
           `∃x. bc_find_loc_aux bce bs.inst_length l 0 = SOME x` by (
             Cases_on`bc_find_loc_aux bce bs.inst_length l 0`>>fs[] >>
@@ -3898,8 +3725,8 @@ val compile_val = store_thm("compile_val",
             first_x_assum(qspec_then`l`mp_tac) >>
             rw[] >> rw[] ) >>
           imp_res_tac bc_find_loc_aux_append_code >>
-          qpat_assum`X = bs.code`(assume_tac o SYM) >>
           fs[] ) >>
+        cheat (*
         qpat_assum`good_ecs x y`mp_tac >>
         simp[good_ecs_def,FEVERY_DEF] >>
         disch_then(qspec_then`l`mp_tac) >>
@@ -3930,11 +3757,23 @@ val compile_val = store_thm("compile_val",
         rpt(first_x_assum(qspec_then`fv`mp_tac)) >>
         simp[] >>
         Q.PAT_ABBREV_TAC`P = lookup_ct a b X Y e` >>
-        Cases_on`P`>>simp[DRESTRICT_DEF]) >>
+        Cases_on`P`>>simp[DRESTRICT_DEF] *)) >>
+      reverse conj_asm2_tac >- (
+        simp[SUBMAP_DEF,DRESTRICT_DEF,FDOM_FUPDATE_LIST] >>
+        Cases_on`rs`>>fs[] >>
+        Cases_on`t`>>fs[] >>
+        simp[FUPDATE_LIST_THM] >>
+        simp[FAPPLY_FUPDATE_THM] >>
+        rw[] ) >>
+      match_mp_tac Cenv_bs_change_store >>
+      `∃r. rs = [r]` by (
+        Cases_on`rs`>>fs[] >>
+        Cases_on`t`>>fs[] ) >> fs[FUPDATE_LIST_THM] >>
+      cheat (*
       match_mp_tac Cenv_bs_imp_incsz >>
       qexists_tac`bs with code := bce` >>
-      simp[bc_state_component_equality]) >>
-    Q.ISPECL_THEN[`cd`,`cenv`,`sz`,`0`,`cs`,`[(xs,INR l)]:def list`]mp_tac compile_closures_thm >>
+      simp[bc_state_component_equality] *)) >>
+    Q.ISPECL_THEN[`c`,`cenv`,`sz`,`cs`,`[INR l]:def list`]mp_tac compile_closures_thm >>
     simp[] >> disch_then strip_assume_tac >>
     pop_assum kall_tac >>
     fs[Once SWAP_REVERSE] >>
@@ -3945,43 +3784,38 @@ val compile_val = store_thm("compile_val",
     simp[] >>
     qexists_tac`REVERSE args`>>fs[EVERY2_EVERY]) >>
   strip_tac >- (
-    simp[] >> rpt gen_tac >> strip_tac >>
+    simp[] >> ntac 6 gen_tac >> qx_gen_tac `fenv` >> rpt gen_tac >> strip_tac >>
     rpt gen_tac >>
     simp[compile_def,FOLDL_UNION_BIGUNION] >>
     simp_tac(srw_ss()++ETA_ss)[] >>
     strip_tac >> rfs[] >> fs[] >>
     BasicProvers.VAR_EQ_TAC >>
-    qspecl_then[`cd`,`cenv`,`TCNonTail F`,`sz`,`cs`,`exp`](Q.X_CHOOSE_THEN`cx`strip_assume_tac)(CONJUNCT1 compile_append_out) >> fs[] >>
+    qspecl_then[`c`,`cenv`,`TCNonTail F`,`sz`,`cs`,`exp`](Q.X_CHOOSE_THEN`cx`strip_assume_tac)(CONJUNCT1 compile_append_out) >> fs[] >>
     simp[GSYM FORALL_AND_THM] >> ntac 2 gen_tac >>
-    Q.PAT_ABBREV_TAC`cs0 = compile cd cenv X sz cs exp` >>
-    qspecl_then[`cd`,`cenv`,`sz+1`,`cs0`,`exps`](Q.X_CHOOSE_THEN`cxs`strip_assume_tac)(CONJUNCT2 (CONJUNCT2 compile_append_out)) >> fs[] >>
+    Q.PAT_ABBREV_TAC`cs0 = compile c cenv X sz cs exp` >>
+    qspecl_then[`c`,`cenv`,`sz+1`,`cs0`,`exps`](Q.X_CHOOSE_THEN`cxs`strip_assume_tac)(CONJUNCT2 (CONJUNCT2 compile_append_out)) >> fs[] >>
     reverse(Cases_on`∃bc10. code = REVERSE cx ++ REVERSE cxs ++ bc10`) >- (
       fsrw_tac[DNF_ss][] >>
       conj_tac >> rpt gen_tac >>
       rw[Once SWAP_REVERSE]) >> fs[] >>
     reverse(Cases_on`bs.code = bc0 ++ REVERSE cx ++ REVERSE cxs ++ bc10 ++ bc1`) >- fs[] >>
     fs[Once SWAP_REVERSE] >>
-    POP_ASSUM_LIST(map_every assume_tac) >>
-    first_x_assum(qspecl_then[`rd`,`cs`,`cd`,`cenv`,`sz`,`bs`,`bce`,`bcr`,`bc0`]mp_tac) >>
-    `FDOM s ⊆ FDOM s' ∧ FDOM s' ⊆ FDOM s'' ∧ FDOM s'' ⊆ FDOM s'''` by PROVE_TAC[Cevaluate_store_SUBSET,FST] >>
+    last_x_assum(qspecl_then[`rd`,`cs`,`cenv`,`sz`,`bs`,`bce`,`bcr`,`bc0`]mp_tac) >>
+    `LENGTH s ≤ LENGTH s' ∧ LENGTH s' ≤ LENGTH s'' ∧ LENGTH s'' ≤ LENGTH s'''` by PROVE_TAC[Cevaluate_store_SUBSET,FST] >>
     fs[ALL_DISTINCT_APPEND] >>
     fs[Once SWAP_REVERSE] >>
     disch_then(mp_tac o SIMP_RULE(srw_ss()++DNF_ss)[code_for_push_def,LET_THM] o CONJUNCT1) >>
     disch_then(qx_choosel_then[`rf`,`rd'`,`bf`]strip_assume_tac) >>
     qmatch_assum_abbrev_tac`bc_next^* bs bs1` >>
-    first_x_assum(qspecl_then[`rd'`,`cs0`,`cd`,`cenv`,`sz+1`,`bs1`,`bce`,`bcr`,`bc0 ++ REVERSE cx`,`REVERSE cxs`]mp_tac) >>
+    first_x_assum(qspecl_then[`rd'`,`cs0`,`cenv`,`sz+1`,`bs1`,`bce`,`bcr`,`bc0 ++ REVERSE cx`,`REVERSE cxs`]mp_tac) >>
     simp[Abbr`bs1`] >>
-    qmatch_abbrev_tac`(P ⇒ Q) ⇒ R` >>
-    `P` by (
-      map_every qunabbrev_tac[`P`,`Q`,`R`] >>
+    discharge_hyps >- (
       simp[Abbr`cs0`] >>
-      conj_tac >- PROVE_TAC[SUBSET_TRANS] >>
+      conj_tac >- PROVE_TAC[SUBSET_DEF,IN_COUNT,LESS_LESS_EQ_TRANS] >>
       conj_tac >- metis_tac[Cevaluate_Clocs,FST] >>
       match_mp_tac compile_labels_lemma >>
-      map_every qexists_tac [`cd`,`cenv`,`TCNonTail F`,`sz`,`cs`,`exp`,`bc0`,`REVERSE cx`] >>
+      map_every qexists_tac [`c`,`cenv`,`TCNonTail F`,`sz`,`cs`,`exp`,`bc0`,`REVERSE cx`] >>
       rw[] ) >>
-    simp[] >>
-    map_every qunabbrev_tac[`P`,`Q`,`R`] >>
     disch_then(mp_tac o SIMP_RULE(srw_ss()++DNF_ss)[code_for_push_def,LET_THM]) >>
     disch_then(qx_choosel_then[`bvs`,`rfs`,`rd''`]strip_assume_tac) >>
     conj_tac >- (
@@ -3994,9 +3828,7 @@ val compile_val = store_thm("compile_val",
         fs[Cenv_bs_def,s_refs_def,good_rd_def,FEVERY_DEF,UNCURRY,SUBMAP_DEF,SUBSET_DEF]) >>
       pop_assum mp_tac >>
       simp[Abbr`cl`,Once Cv_bv_cases] >>
-      disch_then(qx_choosel_then[`a`,`bve`,`b`,`i'`,`l`,`xs'`]strip_assume_tac) >>
-      `(i' = i) ∧ (xs' = xs)` by ( Cases_on`ns = []` >> fs[] >> rfs[]) >> rw[] >>
-      fs[] >> rfs[] >> rw[] >> fs[] >> rw[] >>
+      disch_then(qx_choosel_then[`a`,`bve`,`cd`,`l`]strip_assume_tac) >>
       qho_match_abbrev_tac`∃rf sm bv. bc_next^* bs (bs2 rf bv) ∧ P rf sm bv` >>
       qmatch_assum_abbrev_tac`bc_next^* bs0 bs3` >>
       qmatch_assum_abbrev_tac`bc_next^* bs0 bs3` >>
@@ -4075,72 +3907,41 @@ val compile_val = store_thm("compile_val",
       qpat_assum`bc_fetch X = Y` kall_tac >>
       Q.PAT_ABBREV_TAC`ret = x + 1` >>
       qho_match_abbrev_tac`∃rf sm bv. bc_next^* bs1 (bs2 rf bv) ∧ P rf sm bv` >>
-      qpat_assum`good_code_env c d bce`(fn th => mp_tac((uncurry CONJ)((I##Q.SPEC`l`)(CONJ_PAIR(SIMP_RULE(srw_ss())[good_code_env_def,FEVERY_DEF]th)))) >> assume_tac th) >>
-      fs[FLOOKUP_DEF] >>
-      `cb = INR l` by ( Cases_on`ns=[]`>>fs[]>>rfs[] ) >> fs[] >>
-      simp_tac(srw_ss()++DNF_ss)[] >>
-      qpat_assum`X = d ' l`(assume_tac o SYM) >>
-      simp[] >>
-      map_every qx_gen_tac [`cdc`,`csc`,`cb0`,`cc`,`cb1`] >>
+      rator_assum`code_env_code`(mp_tac o SIMP_RULE(srw_ss())[FEVERY_DEF,code_env_code_def]) >>
       strip_tac >>
+      first_x_assum(qspec_then`l`mp_tac) >>
+      fs[FLOOKUP_DEF] >>
+      disch_then(qx_choosel_then[`csc`,`cb0`,`cc`,`cb1`] strip_assume_tac) >>
       pop_assum (assume_tac o SYM) >>
-      qmatch_assum_abbrev_tac`cdc.env_azs ' l = (enc,LENGTH vs)` >>
-      first_x_assum (qspecl_then[`rd''`,`csc`,`cdc`,`enc`,`0`,`bs1`,`bce`,`bcr`,`cb0 ++ [Label l]`]mp_tac) >>
+      fs[el_check_def] >>
+      `∃recs envs. cd.ceenv = (recs,envs)` by (Cases_on`cd.ceenv`>>simp[]>>PROVE_TAC[]) >> fs[] >>
+      first_x_assum (qspecl_then[`rd''`,`csc`,`MAP CTEnv cd.ccenv`,`0`,`bs1`,`bce`,`bcr`,`cb0 ++ [Label l]`]mp_tac) >>
       simp[] >>
-      qmatch_abbrev_tac`(X ⇒ Q) ⇒ R` >>
-      `X` by (
-        map_every qunabbrev_tac[`X`,`P`,`Q`,`R`] >>
-        `(ns ≠ [] ⇒ i < LENGTH ns) ∧ ALL_DISTINCT ns` by (
-          Cases_on`ns=[]`>>fs[] >>
-          imp_res_tac find_index_LESS_LENGTH >> fs[] ) >>
-        simp[FDOM_bind_fv,Abbr`enc`] >>
+      discharge_hyps >- (
+        rator_assum`good_code_env`(mp_tac o SIMP_RULE(srw_ss())[good_code_env_def,IN_FRANGE,GSYM LEFT_FORALL_IMP_THM]) >>
+        disch_then(qspec_then`l`mp_tac) >>
+        simp[closure_data_component_equality] >> strip_tac >>
         conj_tac >- (
-          unabbrev_all_tac >>
-          fs[FLOOKUP_DEF] >> rfs[] >>
-          fs[DISJOINT_DEF,EXTENSION] >> rw[] >>
-          ntac 9 (pop_assum kall_tac) >>
-          ntac 3 (pop_assum (qspec_then`x`mp_tac)) >>
-          Cases_on `x ∈ free_vars c (c ' l)` >> fs[] >>
-          Cases_on `x ∈ set (binders (c ' l))` >> fs[] >>
-          qspecl_then[`c`,`c ' l`,`l`]mp_tac(CONJUNCT1 free_vars_DOMSUB) >>
-          simp[SUBSET_DEF] >>
-          disch_then(qspec_then`x`strip_assume_tac) >> rfs[] >>
-          Cases_on`MEM x ns`>>fs[]>>
-          Cases_on`MEM x ns'`>>fs[]>>
-          qpat_assum`benv_bvs X Y Z ns env' defs ns' i`mp_tac >>
-          simp[Once Cv_bv_cases] >> rw[] >> pop_assum mp_tac >>
-          Q.PAT_ABBREV_TAC`fvs = SET_TO_LIST (free_vars X Y)` >>
-          Q.PAT_ABBREV_TAC`evs = FILTER X fvs` >>
-          `MEM x evs` by (
-            Q.ISPECL_THEN[`ns'`,`x`,`0`]mp_tac find_index_MEM >>
-            simp[Abbr`evs`,MEM_FILTER] >>
-            simp[Abbr`fvs`] ) >>
-          pop_assum(mp_tac o SIMP_RULE std_ss [MEM_EL]) >>
-          disch_then(Q.X_CHOOSE_THEN`z` strip_assume_tac) >>
-          disch_then(qspec_then`z`mp_tac) >> simp[] >>
-          Q.ISPECL_THEN[`ns'`,`x`,`0`]mp_tac find_index_MEM >>
-          simp[] ) >>
-        conj_tac >- (
-          qspecl_then[`c`,`d`,`s`,`env`,`exp`,`(s',Rval (CRecClos env' ns defs n))`]mp_tac (CONJUNCT1 Cevaluate_Clocs) >>
-          qspecl_then[`c`,`d`,`s'`,`env`,`exps`,`(s'',Rval vs)`]mp_tac (CONJUNCT2 Cevaluate_Clocs) >>
+          qspecl_then[`c`,`s`,`env`,`exp`,`(s',Rval (CRecClos fenv defs cd.ix))`]mp_tac (CONJUNCT1 Cevaluate_Clocs) >>
+          qspecl_then[`c`,`s'`,`env`,`exps`,`(s'',Rval vs)`]mp_tac (CONJUNCT2 Cevaluate_Clocs) >>
           simp[] >>
-          qpat_assum `LENGTH xs = LENGTH vs` mp_tac >>
-          qpat_assum `FDOM s' ⊆ FDOM s''` mp_tac >>
+          rpt (qpat_assum `X ⊆ count (LENGTH s)`mp_tac) >>
+          rpt(qpat_assum `LENGTH X ≤ LENGTH Y` mp_tac) >>
+          qpat_assum `LENGTH fenv = X`mp_tac >>
+          qpat_assum `EVERY Z envs` mp_tac >>
           rpt (pop_assum kall_tac) >>
-          fsrw_tac[DNF_ss][extend_rec_env_def,SUBSET_DEF,FOLDL2_FUPDATE_LIST,FOLDL_FUPDATE_LIST,MAP2_MAP,FST_pair,SND_pair,MAP_ZIP] >>
-          qx_gen_tac `x` >>
-          simp[FORALL_AND_THM,RIGHT_FORALL_IMP_THM] >>
-          ntac 4 strip_tac >>
-          simp[Once CONJ_COMM] >> simp[GSYM AND_IMP_INTRO] >>
-          ho_match_mp_tac IN_FRANGE_FUPDATE_LIST_suff >>
-          reverse conj_tac >-
-            (srw_tac[DNF_ss][MAP_ZIP] >> PROVE_TAC[]) >>
-          ho_match_mp_tac IN_FRANGE_FUPDATE_LIST_suff >>
-          srw_tac[DNF_ss][MAP_MAP_o,combinTheory.o_DEF,MEM_MAP] >>
-          PROVE_TAC[] ) >>
-        conj_tac >- metis_tac[Cevaluate_Clocs,FST] >>
-        conj_tac >- simp[Abbr`bs1`] >>
+          ntac 9 strip_tac  >>
+          fsrw_tac[DNF_ss][SUBSET_DEF,MEM_MAP,EVERY_MEM] >>
+          metis_tac[LESS_LESS_EQ_TRANS,MEM_EL] ) >>
         conj_tac >- (
+          qspecl_then[`c`,`s`,`env`,`exp`,`(s',Rval (CRecClos fenv defs cd.ix))`]mp_tac (CONJUNCT1 Cevaluate_Clocs) >>
+          qspecl_then[`c`,`s'`,`env`,`exps`,`(s'',Rval vs)`]mp_tac (CONJUNCT2 Cevaluate_Clocs) >>
+          simp[] >> strip_tac >> strip_tac >>
+          fsrw_tac[DNF_ss][] >>
+          first_x_assum match_mp_tac >>
+          metis_tac[SUBSET_DEF,IN_COUNT,LESS_LESS_EQ_TRANS] ) >>
+        conj_tac >- simp[Abbr`bs1`] >>
+        conj_asm1_tac >- (
           fs[Abbr`bs1`,Abbr`l2a`] >>
           qspecl_then[`bce`,`bs.inst_length`,`l`,`0`]mp_tac bc_find_loc_aux_ALL_DISTINCT >>
           simp[] >>
@@ -4152,35 +3953,41 @@ val compile_val = store_thm("compile_val",
           simp[FILTER_APPEND] ) >>
         conj_tac >- (
           match_mp_tac Cenv_bs_bind_fv >>
-          map_every qexists_tac[`env'`,`defs`,`b`,`l`,`vs`] >>
-          simp[Abbr`bs1`] >>
-          map_every qexists_tac[`a`,`bvs`,`bs.stack`] >>
           simp[] >>
-          conj_tac >- ( fs[s_refs_def,Cenv_bs_def,good_rd_def] ) >>
-          conj_tac >- (rw[] >> fs[]) >>
-          conj_tac >- (rw[] >> fs[]) >>
-          fs[FLOOKUP_DEF] >> rfs[] >>
-          fs[Abbr`l2a`] >>
-          match_mp_tac (GEN_ALL benv_bvs_free_vars_SUBSET) >>
-          simp[] >> metis_tac[] ) >>
+          qexists_tac`cd`>>simp[]>>
+          qexists_tac`e`>>simp[]>>
+          simp[Abbr`bs1`]>>
+          map_every qexists_tac[`bvs`,`a`,`bs.stack`] >> simp[] >>
+          map_every qexists_tac[`vs`,`fenv`,`defs`] >> simp[] >>
+          map_every qexists_tac[`envs`,`recs`] >> simp[] >>
+          simp[FLOOKUP_DEF] >>
+          simp[closure_data_component_equality] >>
+          conj_tac >- metis_tac[] >>
+          fs[s_refs_def,Cenv_bs_def,good_rd_def] >>
+          qspecl_then[`bce`,`bs.inst_length`,`l`,`0`]mp_tac bc_find_loc_aux_ALL_DISTINCT >>
+          simp[] >>
+          disch_then(qspec_then`LENGTH cb0`mp_tac) >>
+          srw_tac[ARITH_ss][] >>
+          pop_assum mp_tac >>
+          REWRITE_TAC[GSYM APPEND_ASSOC] >>
+          rw[EL_LENGTH_APPEND,TAKE_LENGTH_APPEND] >>
+          simp[FILTER_APPEND] ) >>
         qpat_assum`X = bce`(assume_tac o SYM) >>
         fs[ALL_DISTINCT_APPEND,FILTER_APPEND] ) >>
-      simp[] >>
-      map_every qunabbrev_tac[`X`,`Q`] >>
-      disch_then(qspecl_then[`0`,`LENGTH vs`]mp_tac o CONV_RULE (RESORT_FORALL_CONV List.rev) o CONJUNCT2) >>
+      disch_then(qspecl_then[`0`,`cd.az`]mp_tac o CONV_RULE (RESORT_FORALL_CONV List.rev) o CONJUNCT2) >>
       simp[] >> simp[Once SWAP_REVERSE] >>
       simp_tac (srw_ss()++DNF_ss) [] >>
       disch_then(mp_tac o CONV_RULE (RESORT_FORALL_CONV List.rev)) >>
       simp[LENGTH_NIL_SYM,FUPDATE_LIST_THM] >>
       simp_tac(srw_ss())[Abbr`bs1`]>>
-      disch_then(qspecl_then[`bs.stack`,`Block 3 [CodePtr a; Block 0 bve]`,`bvs`,`vs`,`xs`,`defs`,`ns`,`env'`]mp_tac) >>
-      pop_assum kall_tac >>
-      `LENGTH bvs = LENGTH vs` by fs[EVERY2_EVERY] >>
+      disch_then(qspecl_then[`bs.stack`,`Block 3 [CodePtr a; Block 0 bve]`,`bvs`,`vs`]mp_tac) >>
       `∃bc10. bs.code = cb0 ++ [Label l] ++ REVERSE cc ++ bc10` by (
         qpat_assum`bce ++ bcr = X`(assume_tac o SYM) >>
         qpat_assum`X = bce`(assume_tac o SYM) >>
         rw[] ) >> pop_assum SUBST1_TAC >> fs[] >>
-      simp[code_for_return_def,Abbr`R`] >>
+      `LENGTH bvs = LENGTH vs` by fs[EVERY2_EVERY] >>
+      simp[] >>
+      simp[code_for_return_def] >>
       disch_then(qx_choosel_then[`bvr`,`rfr`,`smr`]strip_assume_tac) >>
       map_every qexists_tac [`rfr`,`smr`,`bvr`] >>
       simp[Abbr`bs2`] >>
@@ -4190,7 +3997,7 @@ val compile_val = store_thm("compile_val",
         srw_tac[ARITH_ss][FILTER_APPEND,SUM_APPEND,ADD1] ) >>
       rw[] >>
       simp[Abbr`P`] >>
-      reverse conj_tac >- PROVE_TAC[SUBMAP_TRANS] >>
+      reverse conj_tac >- PROVE_TAC[SUBMAP_TRANS,IS_PREFIX_TRANS] >>
       match_mp_tac Cenv_bs_imp_incsz >>
       qunabbrev_tac`bs0` >>
       qmatch_assum_abbrev_tac`Cenv_bs c rd s renv cenv sz bs0` >>
@@ -4203,7 +4010,7 @@ val compile_val = store_thm("compile_val",
       fs[s_refs_def,Abbr`l2a`,good_rd_def] >>
       simp[Abbr`bs0`,bc_state_component_equality] >>
       conj_tac >- metis_tac[SUBMAP_TRANS] >>
-      conj_tac >- metis_tac[SUBMAP_TRANS] >>
+      conj_tac >- metis_tac[IS_PREFIX_TRANS] >>
       fs[Cenv_bs_def,s_refs_def,good_rd_def] >>
       metis_tac[SUBMAP_TRANS]) >>
     asm_simp_tac(srw_ss()++DNF_ss)[] >>
